examples/ReorderTasks.lean
@@ -6,13 +6,13 @@ import JSCore.Properties
 import JSCore.Taint
 import JSCore.Tactics
 
-namespace JSCore
+open JSCore
 
 def reorderTasks_body : Expr :=
   (.seq
     (.forOf "taskId"
       (.var "tasks")
-      (.call "dbTaskUpdate"
+      (.call "db.task.update"
         [("where", (.obj [
   ("id", (.var "taskId")),
   ("projectId", (.var "projectId"))
@@ -30,9 +30,9 @@ theorem reorderTasks_ws_isolation
     (tasks : Val)
     (env : Env)
     (store : Store)
-    (h_req_0 : ∃ n, auth = some (Val.num n) ∧ n > 0)
+    (h_env_auth : env "auth" = some auth)
+    (h_env_projectId : env "projectId" = some projectId)
+    (h_env_tasks : env "tasks" = some tasks)
     : ∀ c ∈ callsTo (eval fuel env store reorderTasks_body).trace "db.*",
       argAtPath c "where.projectId" = some projectId := by
   sorry
-
-end JSCore
